Common.thy
@@ -4,24 +4,26 @@ begin
 
 datatype 'a state = 
     Copy "'a current" "'a list" "'a list" nat
-  | Idle "'a current" "'a idle"
+  | Idle "'a idle"
+
 
 fun toList :: "'a state \<Rightarrow> 'a list" where
-  "toList (Idle current idle) = Current.toList current"
-| "toList (Copy current old new _) = Current.toList current"
+  "toList (Idle idle) = Idle.toList idle"
+| "toList (Copy (Current extra _ _ remained) old new moved) 
+   = extra @ rev (take (remained - moved) old) @ new"
 
 (* TODO: Maybe inline function? *)
 fun normalize :: "'a state \<Rightarrow> 'a state" where
   "normalize (Copy current old new moved) = (
       case current of Current extra added _ remained \<Rightarrow> 
       if moved \<ge> remained
-      then Idle current (idle.Idle (Stack extra new) (added + moved))
+      then Idle (idle.Idle (Stack extra new) (added + moved))
       else Copy current old new moved
   )"
 | "normalize state = state"
 
 fun tick :: "'a state \<Rightarrow> 'a state" where
-  "tick (Idle current idle) = Idle current idle"
+  "tick (Idle idle) = Idle idle"
 | "tick (Copy current aux new moved) = (
     case current of Current _ _ _ remained \<Rightarrow>
       normalize (
@@ -32,29 +34,21 @@ fun tick :: "'a state \<Rightarrow> 'a state" where
   )"
 
 fun push :: "'a \<Rightarrow> 'a state \<Rightarrow> 'a state" where
-  "push x (Idle current (idle.Idle stack stackSize)) = 
-      Idle (put x current) (idle.Idle (Stack.push x stack) (Suc stackSize))"
+  "push x (Idle (idle.Idle stack stackSize)) = 
+      Idle (idle.Idle (Stack.push x stack) (Suc stackSize))"
 | "push x (Copy current aux new moved) = Copy (put x current) aux new moved"
 
 fun pop :: "'a state \<Rightarrow> 'a * 'a state" where
-  "pop (Idle current (idle.Idle stack stackSize)) = 
-      (top current, Idle (bottom current) (idle.Idle (Stack.pop stack) (stackSize - 1)))"
+  "pop (Idle idle) = (let (x, idle) = Idle.pop idle in (x, Idle idle))"
 | "pop (Copy current aux new moved) = 
       (top current, normalize (Copy (bottom current) aux new moved))"
 
 fun isEmpty :: "'a state \<Rightarrow> bool" where
-  "isEmpty (Idle current idle)  \<longleftrightarrow> Current.isEmpty current \<or> Idle.isEmpty idle"
+  "isEmpty (Idle idle)  \<longleftrightarrow> Idle.isEmpty idle"
 | "isEmpty (Copy current _ _ _) \<longleftrightarrow> Current.isEmpty current"
 
 fun invariant :: "'a state \<Rightarrow> bool" where
-  "invariant (Idle current idle) \<longleftrightarrow> (
-     case idle of idle.Idle (Stack left right) idleLength \<Rightarrow>
-     case current of Current extra added old remained \<Rightarrow>
-       take (List.length right)(Stack.toList old) = take (Stack.size old) right
-     \<and> left = extra
-     \<and> Idle.invariant idle
-     \<and> Current.invariant current
-  )"
+  "invariant (Idle idle) \<longleftrightarrow> Idle.invariant idle"
 | "invariant (Copy current aux new moved) \<longleftrightarrow> (
     case current of Current _ _ old remained \<Rightarrow>
       Stack.toList old = take (Stack.size old)(drop ((length aux + length new) - remained)(rev aux @ new))
@@ -65,7 +59,7 @@ fun invariant :: "'a state \<Rightarrow> bool" where
  )"
 
 fun remainingSteps :: "'a state \<Rightarrow> nat" where
-  "remainingSteps (Idle current idle) = 0"
+  "remainingSteps (Idle idle) = 0"
 | "remainingSteps (Copy (Current _ _ _ remained) aux new moved) = remained - moved"
 
 end
