Common_Proof.thy
@@ -2,29 +2,100 @@ theory Common_Proof
   imports Common Idle_Proof Current_Proof
 begin
 
-lemma tick: "toList (tick common) = toList common"
-  apply(induction common)
-  by(auto split: current.splits)
-
-lemma tick_2: "Common.tick common = common' \<Longrightarrow> Common.toList common = Common.toList common'"
-  by(auto simp: tick)
-
-lemma pop: "\<lbrakk>\<not> isEmpty common; pop common = (x, common')\<rbrakk> \<Longrightarrow> x # toList common' = toList common"
-  apply(induction common arbitrary: x rule: pop.induct)
-   apply(auto simp: get  split: prod.splits current.splits if_splits)
-  using get by fastforce+
-
-lemma push: "toList (push x common) = x # toList common"
-  apply(induction x common rule: push.induct)
-  by(auto simp: put)
-
 lemma take_hd: "xs \<noteq> [] \<Longrightarrow> take (Suc 0) xs = [hd xs]"
   apply(induction xs)
   by auto
- 
+
+lemma helping_1_1: "\<lbrakk>a \<le> Suc b; b < a\<rbrakk> \<Longrightarrow> a - b = 1"
+  by auto
+
+lemma helping_1: "\<lbrakk>
+  Stack.toList x3b = take (Stack.size x3b) (drop (length x2 + length x3 - x4) (rev x2)) @ take (Stack.size x3b + length x3 - x4) x3;
+  x4 \<le> length x2 + length x3; 
+  x4 \<le> Suc (length x3); 
+  length x3 < x4
+\<rbrakk> \<Longrightarrow> take (x4 - length x3) x2 = [hd x2]"
+  apply(auto simp: helping_1_1)
+  apply(induction x2)
+  by auto
+
+lemma helping_2: "\<lbrakk>
+  Stack.toList x3b = take (Stack.size x3b) (drop (length x2 + length x3 - x4) (rev x2)) @ take (Stack.size x3b + length x3 - x4) x3;
+  x4 \<le> length x2 + length x3; 
+  \<not> x4 \<le> Suc (length x3)
+\<rbrakk> \<Longrightarrow> rev (take (x4 - Suc (length x3)) (tl x2)) @ [hd x2] = rev (take (x4 - length x3) x2)"
+  (* TODO:* *)
+  by (metis Suc_diff_Suc le_SucI length_greater_0_conv less_add_same_cancel2 less_le_trans not_le_imp_less rev.simps(2) take_Suc)
+
+lemma tick: "invariant common \<Longrightarrow> toList (tick common) = toList common"
+  apply(induction common)
+  by(auto simp: take_hd helping_1 helping_2  split: current.splits)
+
+lemma tick_2: "invariant common \<Longrightarrow> tick common = common' \<Longrightarrow> toList common = toList common'" 
+  by(auto simp: tick)
+
+lemma helper_pop_1: "\<lbrakk>remained > length new; remained - Suc 0 \<le> length new\<rbrakk> \<Longrightarrow> remained - length new = 1"
+  by auto
+
+lemma helper_pop_2: "\<lbrakk>
+  \<not> remained \<le> length new; \<not> Stack.isEmpty old;
+  Stack.toList old =
+  take (Stack.size old) (drop (length aux + length new - remained) (rev aux)) @ take (Stack.size old + length new - remained) new;
+  x = first old;
+  common' = Copy (Current [] 0 (Stack.pop old) (remained - Suc 0)) aux new (length new); moved = length new;
+  remained \<le> length aux + length new; added = 0;
+  \<not> remained - Suc 0 \<le> length new
+\<rbrakk> \<Longrightarrow> first old # drop (Suc (length aux + length new) - remained) (rev aux) = 
+      drop (length aux + length new - remained) (rev aux)"
+  apply(induction old rule: Stack.pop.induct)
+    apply(auto simp: )
+  apply (smt (verit, ccfv_threshold) Cons_nth_drop_Suc Nat.diff_diff_right Suc_diff_le add_Suc append_Cons append_Nil2 diff_diff_cancel diff_is_0_eq hd_take length_drop length_rev list.sel(1) nat_le_linear not_le take_all_iff take_eq_Nil zero_less_Suc)
+  by (smt (verit, ccfv_threshold) Cons_nth_drop_Suc Nat.diff_diff_right Nil_is_append_conv Stack.toList.simps Suc_diff_le add_Suc append_Cons append_Nil2 diff_diff_cancel diff_is_0_eq drop_all_iff empty first hd_take le_diff_conv length_drop length_rev list.sel(1) nat_le_linear not_le self_append_conv2 take_all_iff take_eq_Nil zero_less_Suc)
+
+
+lemma pop: "\<lbrakk>invariant common; \<not> isEmpty common; pop common = (x, common')\<rbrakk>
+   \<Longrightarrow> x # toList common' = toList common"
+proof(induction common arbitrary: x rule: pop.induct)
+  case (1 idle)
+  then show ?case 
+    by(auto simp: Idle_Proof.pop split: prod.splits)
+next
+  case (2 current aux new moved)
+  then show ?case
+  proof(induction current rule: get.induct)
+    case (1 added old remained)
+    then show ?case 
+    proof(induction "moved \<ge> remained")
+      case True
+      then show ?case by auto
+    next
+      case False
+      then show ?case
+        apply(auto simp: rev_take helper_pop_2 helper_pop_1)
+        by (smt (verit, best) Suc_pred add.commute add_diff_cancel_right' append.right_neutral append_eq_Cons_conv append_eq_conv_conj cancel_comm_monoid_add_class.diff_cancel diff_diff_cancel diff_is_0_eq' dual_order.trans first hd_take helping_1 le_0_eq le_add1 le_add2 le_diff_conv le_diff_iff le_less_Suc_eq length_drop length_greater_0_conv length_rev lessI linear list.size(3) not_empty_2 not_le_imp_less not_less_eq_eq ordered_cancel_comm_monoid_diff_class.diff_diff_right rev.simps(1) rev.simps(2) rev_take size_listLength take_Nil take_all take_all_iff take_eq_Nil take_hd)
+    qed
+  next
+    case (2 x xs added old remained)
+    then show ?case by auto
+  qed
+qed
+
+
+lemma push: "toList (push x common) = x # toList common"
+proof(induction x common rule: push.induct)
+  case (1 x stack stackSize)
+  then show ?case by(auto simp: Stack_Proof.push)
+next
+  case (2 x current aux new moved)
+  then show ?case 
+    apply(induction x current rule: put.induct)
+    by auto
+qed
+
+
 lemma invariant_tick: "invariant common \<Longrightarrow> invariant (tick common)" 
 proof(induction "common" rule: invariant.induct)
-  case (1 current idle)
+  case (1 idle)
   then show ?case
     by auto
 next
@@ -40,16 +111,15 @@ next
     next
       case (Cons a as)
       then show ?case
-        apply auto
-       (* TODO: *)
-        by (metis length_Cons length_take size_listLength)
+        by auto
      qed
   qed
 qed
+
   
 lemma invariant_push: "invariant common \<Longrightarrow> invariant (push x common)"
   apply(induction x common rule: push.induct)
-  by(auto split: stack.splits current.splits)
+  by(auto simp: Stack_Proof.size_push split: stack.splits current.splits)
 
 lemma helper_x: " \<not> Stack.isEmpty stack \<Longrightarrow> Suc (Stack.size (Stack.pop stack) + x) = Stack.size stack + x"
   apply(induction stack rule: Stack.pop.induct)
@@ -84,45 +154,35 @@ lemma invariant_pop: "\<lbrakk>
   pop common = (x, common')
 \<rbrakk> \<Longrightarrow> invariant common'"
 proof(induction common arbitrary: x rule: pop.induct)
-  case (1 current stack stackSize)
-  then show ?case
-  proof(induction current rule: get.induct)
-    case (1 added old remained)
-    then show ?case
-      apply(auto split: stack.splits current.splits prod.splits)
-      apply (metis Stack.pop.simps(2) Stack.toList.simps Stack_Proof.pop append.left_neutral first_pop length_Cons size_listLength stack.inject take_tl)
-      using Stack.isEmpty.simps(1) Stack.pop.elims 
-       apply blast
-      using Stack_Proof.size_pop by fastforce
-  next
-    case (2 x xs added old remained)
-    then show ?case by(auto split: stack.splits current.splits prod.splits)
-  qed
+  case (1 idle)
+  then show ?case 
+    by(auto simp: invariant_pop split: prod.splits)
 next
   case (2 current aux new moved)
-  then show ?case
+  then show ?case 
   proof(induction current rule: get.induct)
     case (1 added old remained)
     then show ?case
-    proof(induction "length new < Stack.size (Stack.pop old)")
-      case True
-      then show ?case 
+    proof(induction old rule: Stack.pop.induct)
+      case (1 x left right)
+      then show ?case
         apply auto
-        apply (smt (verit) Nat.add_0_right Nat.diff_diff_right Stack_Proof.pop Stack_Proof.size_pop Suc_diff_Suc Suc_diff_diff Suc_diff_le Suc_leI add_Suc_right append.right_neutral append_Nil2 append_take_drop_id bot_nat_0.extremum diff_Suc_Suc diff_add_inverse diff_diff_cancel diff_diff_left diff_is_0_eq' first_pop le0 le_diff_conv length_Cons length_append length_drop length_rev less_or_eq_imp_le list.size(3) list.size(3) nat.inject nat_less_le nat_neq_iff not_le old.nat.inject size_listLength)
-        apply(simp add: helper_y)
-        by (meson diff_le_self le_trans)
+        apply (smt (verit, del_insts) Stack.isEmpty.simps(2) Stack.pop.simps(1) Stack.size.simps Stack.toList.simps append_Cons helper_y length_Cons length_append)
+        by (meson diff_le_self order_trans)
     next
-      case False
+      case (2 x right)
       then show ?case 
         apply auto
-        apply (smt (verit, best) Cons_nth_drop_Suc Stack_Proof.pop Stack_Proof.size_pop Suc_pred add_diff_cancel_right' append_Nil2 append_eq_append_conv2 diff_diff_cancel diff_diff_left diff_is_0_eq' le_diff_conv length_0_conv length_drop length_rev less_imp_le list.sel(3) not_le ordered_cancel_comm_monoid_diff_class.diff_diff_right same_append_eq size_listLength take_all take_eq_Nil tl_append2 zero_less_diff)
-        apply(simp add: helper_y)
-        using diff_le_self dual_order.trans by blast
+        apply (smt (verit) Stack.isEmpty.elims(2) Stack.pop.simps(2) Stack.size.simps Stack.toList.simps add.commute append_Nil gen_length_def helper_x helper_y length_code list.discI list.size(3))
+        by (meson diff_le_self dual_order.trans)
+    next
+      case 3
+      then show ?case by auto
     qed
   next
     case (2 x xs added old remained)
     then show ?case by auto
-  qed   
+  qed
 qed
 
 lemma invariant_ticks: "invariant common \<Longrightarrow> invariant ((tick^^n) common)"
@@ -134,7 +194,7 @@ lemma remainingSteps: "remainingSteps state > 0 \<Longrightarrow> remainingSteps
   by auto
 
 lemma tickN: "invariant state
-   \<Longrightarrow> \<exists>current idle. (tick^^ remainingSteps state) state = Idle current idle"
+   \<Longrightarrow> \<exists> idle. (tick^^ remainingSteps state) state = Idle idle"
 proof(induction "remainingSteps state" arbitrary: state)
 case 0
   then show ?case
@@ -154,7 +214,7 @@ next
   then have "remainingSteps state' = x"
     by (metis Suc.hyps(2) nat.inject remainingSteps state' zero_less_Suc)
 
-  then have "\<exists>current idle. (tick^^ x) state' = Idle current idle"
+  then have "\<exists> idle. (tick^^ x) state' = Idle idle"
     using Suc.hyps(1) \<open>Common.invariant state'\<close> by blast
 
   then show ?case
